minterop.fst
@@ -168,10 +168,10 @@ let incrs1' : int -> M4 int = export incrs1
 let incrs2  : (x:int) -> Pure int (x > 0) (fun (y:int) -> y = x + 1) = fun x -> x + 1
 let incrs2' : int -> M4 int = export incrs2
 
-let _export_IOStHist_arrow_spec #t1 #t2 
-  {| d1:importable t1 |} {| d2:exportable t2 |}
-  (pre : t1 -> events_trace -> Type0)
-  {| checkable2 pre |}
+let _export_IOStHist_arrow_spec 
+  (#t1:Type) {| d1:importable t1 |}
+  (#t2:Type) {| d2:exportable t2 |}
+  (pre : t1 -> events_trace -> Type0) {| checkable2 pre |}
   (post : t1 -> events_trace -> maybe (events_trace * t2) -> events_trace -> Type0)
   (f:(x:t1 -> IOStHist t2 (pre x) (post x))) : 
   Tot (d1.itype -> M4 d2.etype) =
@@ -185,9 +185,40 @@ let _export_IOStHist_arrow_spec #t1 #t2
       | None -> M4.raise Contract_failure)
         
 
-instance exportable_IOStHist_arrow_spec t1 t2 (pre : t1 -> events_trace -> Type0) (post : t1 -> events_trace -> maybe (events_trace * t2) -> events_trace -> Type0)
-  {| d1:importable t1 |} {| d2:exportable t2 |} {| d4:checkable2 pre |} : exportable ((x:t1) -> IOStHist t2 (pre x) (post x)) = 
-  mk_exportable (d1.itype -> M4 d2.etype) (_export_IOStHist_arrow_spec #t1 #t2 pre post)
+instance exportable_IOStHist_arrow_spec 
+  (t1:Type) {| d1:importable t1 |} 
+  (t2:Type) {| d2:exportable t2 |}
+  (pre : t1 -> events_trace -> Type0) {| checkable2 pre |}
+  (post : t1 -> events_trace -> maybe (events_trace * t2) -> events_trace -> Type0) :
+  Tot (exportable ((x:t1) -> IOStHist t2 (pre x) (post x))) = 
+    mk_exportable (d1.itype -> M4 d2.etype) (_export_IOStHist_arrow_spec #t1 #d1 #t2 #d2 pre post)
+
+let pre : int -> events_trace -> Type0 = fun x _ -> x = 2
+let post : int -> events_trace -> maybe (events_trace * int) -> events_trace -> Type0 = fun x _ _ _ -> x == 2
+
+val f : (x:int) -> IOStHist int (pre x) (post x)
+let f (x:int) = 5
+
+val f' : int -> M4 int
+let f' = _export_IOStHist_arrow_spec pre post f
+
+// TODO: why is this failing?
+// let f'' = export f
+
+instance exportable_GIO_arrow_spec 
+  (t1:Type) {| d1:importable t1 |} 
+  (t2:Type) {| d2:exportable t2 |}
+  (pi_check:check_type) : 
+  Tot (exportable (t1 -> GIO t2 pi_check)) = 
+  mk_exportable 
+    (d1.itype -> M4 d2.etype) 
+    (_export_IOStHist_arrow_spec (fun _ -> gio_pre pi_check) (fun _ -> gio_post pi_check))
+
+let pis : check_type = fun _ _ -> true
+let g () : GIO int pis = 5
+// TODO: why is this failing?
+// let g' : unit -> M4 int = export g
+
 
     // (fun (f:(x:t1 -> IOStHist t2 (pre x) (post x))) ->
     //   (fun (x:d1.itype) ->
